Test/civl/regression-tests/issue-1085.bpl
@@ -1,12 +1,12 @@
 // RUN: %parallel-boogie "%s" > "%t"
 // RUN: %diff "%s.expect" "%t"
 
-yield procedure {:layer 1} Foo({:linear_in} x: Set (One int), i: int)
-    returns ({:linear} x': Set (One int))
+yield procedure {:layer 1} Foo({:linear_in} x: UnitMap (One int), i: int)
+    returns ({:linear} x': UnitMap (One int))
 requires {:layer 1} Map_Contains(x, One(i));
 refines atomic action _ { x' := x; }
 {
-    var a: Set (One int);
+    var a: UnitMap (One int);
     var b: One int;
 
     b := One(i);
@@ -15,8 +15,8 @@ refines atomic action _ { x' := x; }
     x' := a;
 }
 
-yield procedure {:layer 1} Bar({:linear_in} a: Set (One int), i: int)
-    returns ({:linear} a': Set (One int), {:linear} b: One int)
+yield procedure {:layer 1} Bar({:linear_in} a: UnitMap (One int), i: int)
+    returns ({:linear} a': UnitMap (One int), {:linear} b: One int)
 requires {:layer 1} Map_Contains(a, One(i));
 refines atomic action _ { a' := a; b := One(i); call One_Get(a', b); }
 {
