Test/civl/regression-tests/perm.bpl
@@ -4,10 +4,10 @@
 var {:layer 0,1} x: int;
 
 yield procedure {:layer 1}
-mainE({:linear_in} permVar_in: Set (One int))
+mainE({:linear_in} permVar_in: UnitMap (One int))
 requires call Yield(permVar_in, 0);
 {
-    var permVar_out: Set (One int);
+    var permVar_out: UnitMap (One int);
 
     permVar_out := permVar_in;
 
@@ -15,10 +15,10 @@ requires call Yield(permVar_in, 0);
 }
 
 yield procedure {:layer 1}
-foo({:linear_in} permVar_in: Set (One int))
+foo({:linear_in} permVar_in: UnitMap (One int))
 requires call Yield(permVar_in, 0);
 {
-  var permVar_out: Set (One int);
+  var permVar_out: UnitMap (One int);
   permVar_out := permVar_in;
   call Incr();
   call Yield(permVar_out, 1);
@@ -31,6 +31,6 @@ modifies x;
 yield procedure {:layer 0} Incr();
 refines AtomicIncr;
 
-yield invariant {:layer 1} Yield({:linear} p: Set (One int), v: int);
+yield invariant {:layer 1} Yield({:linear} p: UnitMap (One int), v: int);
 preserves Map_Contains(p, One(1));
 preserves x == v;
