Test/civl/regression-tests/perm3.bpl
@@ -3,16 +3,16 @@
 
 var {:layer 0,1} g:int;
 
-yield procedure {:layer 1} PB({:linear_in} permVar_in: Set (One int))
+yield procedure {:layer 1} PB({:linear_in} permVar_in: UnitMap (One int))
 requires call Yield(permVar_in, 0);
 {
-  var permVar_out: Set (One int);
+  var permVar_out: UnitMap (One int);
   permVar_out := permVar_in;
   call IncrG();
   call Yield(permVar_out, 1);
 }
 
-yield procedure {:layer 1} Main({:linear_in} Permissions: Set (One int))
+yield procedure {:layer 1} Main({:linear_in} Permissions: UnitMap (One int))
 requires {:layer 1} Permissions->dom == Set_Add(Set_Add(Set_Empty(), One(0)), One(1));
 {
   call SetG(0);
@@ -33,6 +33,6 @@ modifies g;
 yield procedure {:layer 0} IncrG();
 refines AtomicIncrG;
 
-yield invariant {:layer 1} Yield({:linear} p: Set (One int), v: int);
+yield invariant {:layer 1} Yield({:linear} p: UnitMap (One int), v: int);
 preserves Map_Contains(p, One(0));
 preserves g == v;
