Test/civl/samples/2pc.bpl
@@ -49,22 +49,22 @@ function noConflicts(xids: [TransactionId]bool, xid: TransactionId) : bool
     !(exists x: TransactionId :: Set_Contains(xids, x) && Conflict[x][xid])
 }
 
-function {:inline} VoteRequests(xid: TransactionId, i: int, j: int) : Set (One VoteRequest)
+function {:inline} VoteRequests(xid: TransactionId, i: int, j: int) : UnitMap (One VoteRequest)
 {
     Map((lambda vr: One VoteRequest :: vr->val->xid == xid &&  i <= vr->val->rid && vr->val->rid <= j), MapConst(Unit()))
 }
 
-function allVoteRequests(xid: TransactionId) : Set (One VoteRequest)
+function allVoteRequests(xid: TransactionId) : UnitMap (One VoteRequest)
 {
     VoteRequests(xid, 1, n)
 }
 
-function remainingVoteRequests(xid: TransactionId, i: int) : Set (One VoteRequest)
+function remainingVoteRequests(xid: TransactionId, i: int) : UnitMap (One VoteRequest)
 {
     VoteRequests(xid, i, n)
 }
 
-yield procedure {:layer 1} TPC({:linear} xid: One TransactionId, {:linear_in} vrs: (Set (One VoteRequest)))
+yield procedure {:layer 1} TPC({:linear} xid: One TransactionId, {:linear_in} vrs: (UnitMap (One VoteRequest)))
 requires {:layer 1} vrs == allVoteRequests(xid->val);
 requires call LockedNoConflicts();
 requires call CommittedSubsetLocked();
@@ -72,7 +72,7 @@ requires call XidNotInCommitted(xid);
 {
     var d: Decision;
     var votes: [ReplicaId]Vote;
-    var vrs': Set (One VoteRequest);
+    var vrs': UnitMap (One VoteRequest);
     var i: int;
 
     d := COMMIT();
@@ -101,7 +101,7 @@ requires call XidNotInCommitted(xid);
     }
 }
 
-yield right procedure {:layer 1} vote_all(xid: TransactionId, {:linear_in} vrs: Set (One VoteRequest), i: int) returns (votes: [ReplicaId]Vote, {:linear} vrs': Set (One VoteRequest))
+yield right procedure {:layer 1} vote_all(xid: TransactionId, {:linear_in} vrs: UnitMap (One VoteRequest), i: int) returns (votes: [ReplicaId]Vote, {:linear} vrs': UnitMap (One VoteRequest))
 requires {:layer 1} vrs == VoteRequests(xid, 1, i);
 ensures {:layer 1} (forall j:int :: 1 <= j && j < i+1 && votes[j] == YES() ==> Set_Contains(locked_transactions[j], xid));
 ensures {:layer 1} vrs' == VoteRequests(xid, 1, i);
@@ -125,7 +125,7 @@ modifies locked_transactions;
     }
 }
 
-yield left procedure {:layer 1} finalize_all(d: Decision, {:linear} xid: One TransactionId, {:linear_in} vrs: Set (One VoteRequest))
+yield left procedure {:layer 1} finalize_all(d: Decision, {:linear} xid: One TransactionId, {:linear_in} vrs: UnitMap (One VoteRequest))
 requires {:layer 1} vrs == allVoteRequests(xid->val);
 requires {:layer 1}  (forall j:int :: {:add_to_pool "J", j} d == COMMIT() &&  1 <= j && j < n+1 ==> Set_Contains(locked_transactions[j], xid->val));
 ensures {:layer 1}  (forall j:int :: d == COMMIT() && 1 <=j && j < n+1 ==> Set_Contains(locked_transactions[j], xid->val));
@@ -137,7 +137,7 @@ modifies locked_transactions;
 {
     var i: int;
     var vr: One VoteRequest;
-    var vrs': Set (One VoteRequest);
+    var vrs': UnitMap (One VoteRequest);
 
     vrs' := vrs;
     i := 1;
